---
title: "Multiplicative Law"
nav_order: 2
parent: "Logarithms"
grand_parent: "Algebra"
has_toc: false
---

# Multiplicative Law

This is the multiplication law

$$log_a(b^x) = x\log_a(b)$$

Because if $$a^{\log_a(b)} = b$$, then $$a^{x\log_a(b)} = (a^{\log_a(b)})^x = b^x$$.
Using $$a^{x\log_a(b)} = b^x$$ and taking the log of both sides, we get

$$
\begin{aligned}
a^{x\log_a(b)} &= b^x \\
\log_a(a^{x\log_a(b)}) &= \log_a(b^x) \\
x\log_a(b) &= \log_a(b^x)
\end{aligned}
$$

Which is our multiplicative law

$$\log_a(b^x) = x\log_a(b)$$

We usually think of this as "taking out" the x from the logarithm.