---
title: "Negative Law"
nav_order: 4
parent: "Indicies"
grand_parent: "Algebra"
has_toc: false
---

# Negative Law

Our final application of our additive law is to define negative exponents. For this I will be a little less algebraic.
Say we want to define $$3^{-1}$$. We would hope that $$3^{-1}\times 3^{1} = 3^{-1 + 1}$$ for the sake of consistency, right?
We also know, from the zero law that $$3^{-1}\times 3^{1} = 3^{-1 + 1} = 3^0 = 1$$, meaning $$3^{-1}\times 3 = 1$$.
3 whats equal 1? 3 thirds, of course! so $$3^{-1}$$ must be a third!
In general,

$$3^{-n}\times 3^n = 3^{-n+n} = 3^0 = 1$$

$$3^{-n}\times 3^n = 1$$

Which rearranges to

$$3^{-n} = \frac{1}{3^n}$$

Which is our negative exponent law.